


\begin{latin}
	\begin{enumerate}
		\item
		\[ 
		s_i = a_i \oplus b_i \oplus E_1'c_i \oplus E_1E_0a_ib_i 
		\quad \text{and} \quad 
		c_{i+1} = (E_0 \oplus a_i)b_i + (E_0 \oplus a_i)c_i + b_ic_i
		\]
		
		
		\[
		\begin{array}{|c|c|c|c|}
			\hline
			E_1 & E_0 & s_i & c_{i+1} \\
			\hline
			0 & 0 & s_i = a_i \oplus b_i \oplus c_i & c_{i+1} = a_ib_i + a_ic_i + b_ic_i \\
			0 & 1 & s_i = a_i \oplus b_i \oplus c_i & c_{i+1} = a_i'b_i + a_i'c_i + b_ic_i \\
			1 & 0 & s_i = a_i \oplus b_i & c_{i+1} = a_ib_i + a_ic_i + b_ic_i \\
			1 & 1 & s_i = a_i \oplus b_i \oplus a_ib_i & c_{i+1} = a_i'b_i + a_i'c_i + b_ic_i \\
			\hline
		\end{array}
		\]
		
		
		
		
		
		\item 
		\[
		\begin{array}{|c|c|c|}
			\hline
			E_1 & E_0 & \text{Function} \\
			\hline
			0 & 0 & \text{Add (A + B)} \\
			0 & 1 & \text{Sub (A - B)} \\
			1 & 0 & \text{XOR (A $\oplus$ B)} \\
			1 & 1 & \text{OR (A + B)} \\
			\hline
		\end{array}
		\]
	\end{enumerate}
\end{latin}
